Algoritmos Aproximados/Envasado.dfy/Algoritmo2AproximadoAux.dfy
@@ -5,14 +5,14 @@ include "EnvasadoKAproximado.dfy"
 //Used locally
 predicate allMoreThanHalfFull(E: nat, I: multiset<multiset<nat>>)
 {
-    (forall M: multiset<nat> | M in I :: SumNat(M) * 2 > E)
+    (forall M: multiset<nat> | M in I :: FSumNat(M) * 2 > E)
 }
 
 //Only one bin in I is less than half full
 //Used locally
 predicate oneLessThanHalfFull(E: nat, I: multiset<multiset<nat>>)
 {
-    (exists M: multiset<nat> :: M in I && SumNat(M) * 2 <= E && (forall M': multiset<nat> | M' in I && SumNat(M') * 2 <= E :: M' == M)) 
+    (exists M: multiset<nat> :: M in I && FSumNat(M) * 2 <= E && (forall M': multiset<nat> | M' in I && FSumNat(M') * 2 <= E :: M' == M)) 
 }
 
 lemma allMoreThanHalfFullImplies2Aproximated(A: multiset<nat>, E: nat, I: multiset<multiset<nat>>)
@@ -20,7 +20,9 @@ requires isEnvasado(A, E, I)
 requires allMoreThanHalfFull(E, I) 
 ensures isKAproximatedBinPacking(A, E, I, 2)
 {
-    
+    //for any BinPacking S, |S| * E >= GSumNat(A)
+    assume forall I': multiset<multiset<nat>> | isEnvasado(A, E, I') :: |I| * E >= GSumNat(A);
+    //if the optimal number of bins is x
     assume false;
 }
 
